[CBPV] More ANF attempts

CBPV/ANF.lean
@@ -96,6 +96,9 @@ def up (σ : Nat → Val) : Nat → Val :=
   var 0 +: (renameVal succ ∘ σ)
 prefix:95 "⇑" => up
 
+theorem upId (σ : Nat → Val) (h : ∀ x, σ x = var x) : ∀ x, (⇑ σ) x = var x := by
+  intro n; cases n <;> simp [h]
+
 theorem upExt (σ τ : Nat → Val) (h : ∀ x, σ x = τ x) : ∀ x, (⇑ σ) x = (⇑ τ) x := by
   intro n; cases n <;> simp [h]
 
@@ -140,6 +143,18 @@ def substCfg (σ : Nat → Val) : Cfg → Cfg
   | letin n m => letin (substCom σ n) (substCfg (⇑ σ) m)
   | case v m₁ m₂ => case (substVal σ v) (substCfg (⇑ σ) m₁) (substCfg (⇑ σ) m₂)
 end
+
+theorem substId σ (h : ∀ x, σ x = var x) :
+  (∀ v, substVal σ v = v) ∧
+  (∀ n, substCom σ n = n) ∧
+  (∀ m, substCfg σ m = m) := by
+  refine ⟨λ v ↦ ?val, λ n ↦ ?com, λ m ↦ ? cfg⟩
+  mutual_induction v, n, m generalizing σ
+  all_goals simp; try repeat' constructor
+  all_goals apply_rules [upId]
+
+def substValId := (substId var (λ _ ↦ rfl)).left
+def substCfgId := (substId var (λ _ ↦ rfl)).right.right
 
 theorem substExt {σ τ} (h : ∀ x, σ x = τ x) :
   (∀ v, substVal σ v = substVal τ v) ∧
@@ -362,6 +377,13 @@ def substK (σ : Nat → Val) : K → K
   | .fst k => .fst (substK σ k)
   | .snd k => .snd (substK σ k)
 
+theorem substKId {k} : substK .var k = k := by
+  induction k
+  case nil => rfl
+  case app ih => simp [substValId _, ih]
+  case letin => simp [-up, substCfgExt (upId _ (λ _ ↦ rfl)), substCfgId]
+  case fst ih | snd ih => simp [ih]
+
 theorem substKExt {σ τ k} (h : ∀ x, σ x = τ x) : substK σ k = substK τ k := by
   induction k <;> simp [-lift]
   case app ih => exact ⟨ANF.substValExt h, ih⟩
@@ -445,6 +467,44 @@ theorem wtPlug {Γ k B₁ B₂} {n : ANF.Com}
   case letin hm => exact .letin h hm
   case fst hn => exact hn (.fst h)
   case snd hn => exact hn (.snd h)
+
+/-* Composing continuations *-/
+
+@[simp]
+def compKCfg (k : K) : Cfg → Cfg
+  | .com n => k [ n ]
+  | .letin n m => .letin n (compKCfg (renameK succ k) m)
+  | .case v m₁ m₂ => .case v (compKCfg (renameK succ k) m₁) (compKCfg (renameK succ k) m₂)
+
+@[simp]
+def compKK (k : K) : K → K
+  | .nil => k
+  | .app v k' => .app v (compKK k k')
+  | .letin m => .letin (compKCfg (renameK succ k) m)
+  | .fst k' => .fst (compKK k k')
+  | .snd k' => .snd (compKK k k')
+
+theorem compKCfgNil {m} : compKCfg .nil m = m := by
+  mutual_induction m
+  case com => rfl
+  case letin ih => simp [ih]
+  case case ih₁ ih₂ => simp [ih₁, ih₂]
+
+theorem renameCompKCfg {ξ m k} : renameCfg ξ (compKCfg k m) = compKCfg (renameK ξ k) (renameCfg ξ m) := by
+  mutual_induction m generalizing ξ k
+  case com => simp [renamePlug]
+  case letin ih => simp [ih, renameKLiftSucc]
+  case case ihm₁ ihm₂ => simp [ihm₁, ihm₂, renameKLiftSucc]
+
+theorem renameCompKK {ξ k₁ k₂} : renameK ξ (compKK k₁ k₂) = compKK (renameK ξ k₁) (renameK ξ k₂) := by
+  induction k₂
+  case nil => simp
+  case app ih | fst ih | snd ih => simp [ih]
+  case letin => simp [renameKLiftSucc, renameCompKCfg]
+
+theorem compPlug {n k₁ k₂} : compKCfg k₁ (k₂ [ n ]) = ((compKK k₁ k₂) [ n ]) := by
+  induction k₂ generalizing n <;> apply_assumption
+
 end ANF
 
 /-* A-normal translation of CBPV *-/
@@ -453,27 +513,27 @@ open Val Com
 
 section
 set_option hygiene false
-local notation:40 "⟦" v:41 "⟧ᵥ" => Aval v
-local notation:40 "⟦" m:41 "⟧ₘ" => Acom .nil m
-local notation:40 "⟦" m:41 "⟧ₘ" k:41 => Acom k m
+local notation:1023 "⟦" v "⟧ᵥ" => Aval v
+local notation:1023 "⟦" m "⟧ₘ" => Acom .nil m
+local notation:1022 "⟦" m "⟧ₘ" k => Acom k m
 mutual
 @[simp]
 def Aval : Val → ANF.Val
   | var x => .var x
   | unit => .unit
-  | inl v => .inl (⟦ v ⟧ᵥ)
-  | inr v => .inr (⟦ v ⟧ᵥ)
-  | thunk m => .thunk (⟦ m ⟧ₘ)
+  | inl v => .inl ⟦ v ⟧ᵥ
+  | inr v => .inr ⟦ v ⟧ᵥ
+  | thunk m => .thunk ⟦ m ⟧ₘ
 
 @[simp]
 def Acom (k : ANF.K) : Com → ANF.Cfg
-  | force v => k [ .force (⟦ v ⟧ᵥ) ]
-  | ret v   => k [ .ret (⟦ v ⟧ᵥ) ]
-  | lam m   => k [ .lam (⟦ m ⟧ₘ) ]
-  | app n v   => ⟦ n ⟧ₘ .app (⟦ v ⟧ᵥ) k
-  | letin n m => ⟦ n ⟧ₘ .letin (⟦ m ⟧ₘ (ANF.renameK succ k))
-  | case v m₁ m₂ => .case (⟦ v ⟧ᵥ) (⟦ m₁ ⟧ₘ (ANF.renameK succ k)) (⟦ m₂ ⟧ₘ (ANF.renameK succ k))
-  | prod m₁ m₂ => k [ .prod (⟦ m₁ ⟧ₘ) (⟦ m₂ ⟧ₘ) ]
+  | force v => k [ .force ⟦ v ⟧ᵥ ]
+  | ret v   => k [ .ret ⟦ v ⟧ᵥ ]
+  | lam m   => k [ .lam ⟦ m ⟧ₘ ]
+  | app n v   => ⟦ n ⟧ₘ .app ⟦ v ⟧ᵥ k
+  | letin n m => ⟦ n ⟧ₘ .letin (⟦ m ⟧ₘ ANF.renameK succ k)
+  | case v m₁ m₂ => .case ⟦ v ⟧ᵥ (⟦ m₁ ⟧ₘ ANF.renameK succ k) (⟦ m₂ ⟧ₘ ANF.renameK succ k)
+  | prod m₁ m₂ => k [ .prod ⟦ m₁ ⟧ₘ ⟦ m₂ ⟧ₘ ]
   | fst n => ⟦ n ⟧ₘ .fst k
   | snd n => ⟦ n ⟧ₘ .snd k
   /- I think this is the A-normalization with join points?
@@ -485,18 +545,18 @@ def Acom (k : ANF.K) : Com → ANF.Cfg
   -/
 end
 end
-notation:40 "⟦" v:41 "⟧ᵥ" => Aval v
-notation:40 "⟦" m:41 "⟧ₘ" => Acom ANF.K.nil m
-notation:40 "⟦" m:41 "⟧ₘ" k:41 => Acom k m
+notation:1023 "⟦" v "⟧ᵥ" => Aval v
+notation:1023 "⟦" m "⟧ₘ" => Acom ANF.K.nil m
+notation:1022 "⟦" m "⟧ₘ" k => Acom k m
 
 @[reducible, simp] def Asubst (σ : Nat → Val) : Nat → ANF.Val := λ x ↦ ⟦ σ x ⟧ᵥ
-notation:40 "⟦" σ:41 "⟧ₛ" => Asubst σ
+notation:1023 "⟦" σ "⟧ₛ" => Asubst σ
 
 /-* Translation is type preserving *-/
 
 theorem preservation {Γ} :
-  (∀ {v} {A : ValType}, Γ ⊢ v ∶ A → Γ ⊢ₐ (⟦ v ⟧ᵥ) ∶ A) ∧
-  (∀ {k m} {B₁ B₂ : ComType}, Γ ⊢ k ∶ B₁ ⇒ B₂ → Γ ⊢ m ∶ B₁ → Γ ⊢ₐ (⟦ m ⟧ₘ k) ∶ B₂) := by
+  (∀ {v} {A : ValType}, Γ ⊢ v ∶ A → Γ ⊢ₐ ⟦ v ⟧ᵥ ∶ A) ∧
+  (∀ {k m} {B₁ B₂ : ComType}, Γ ⊢ k ∶ B₁ ⇒ B₂ → Γ ⊢ m ∶ B₁ → Γ ⊢ₐ ⟦ m ⟧ₘ k ∶ B₂) := by
   refine ⟨λ h ↦ ?val, λ hk h ↦ ?com⟩
   mutual_induction h, h
   case var mem => exact .var mem
@@ -517,8 +577,8 @@ theorem preservation {Γ} :
 /-* Renaming commutes with translation *-/
 
 theorem renameA {ξ} :
-  (∀ v, (⟦ renameVal ξ v ⟧ᵥ) = ANF.renameVal ξ (⟦ v ⟧ᵥ)) ∧
-  (∀ m k, (⟦ renameCom ξ m ⟧ₘ (ANF.renameK ξ k)) = ANF.renameCfg ξ (⟦ m ⟧ₘ k)) := by
+  (∀ v, ⟦ renameVal ξ v ⟧ᵥ = ANF.renameVal ξ ⟦ v ⟧ᵥ) ∧
+  (∀ m k, (⟦ renameCom ξ m ⟧ₘ ANF.renameK ξ k) = ANF.renameCfg ξ (⟦ m ⟧ₘ k)) := by
   refine ⟨λ v ↦ ?val, λ m k ↦ ?com⟩
   mutual_induction v, m generalizing ξ
   case var | unit => rfl
@@ -536,20 +596,20 @@ theorem renameA {ξ} :
   case prod ihm₁ ihm₂ => simp [← ihm₁, ← ihm₂, ANF.renamePlug]
   case fst ih | snd ih => simp [← ih]
 
-theorem renameAval {ξ v} : (⟦ renameVal ξ v ⟧ᵥ) = ANF.renameVal ξ (⟦ v ⟧ᵥ) := renameA.left v
-theorem renameAcom {ξ m k} : (⟦ renameCom ξ m ⟧ₘ (ANF.renameK ξ k)) = ANF.renameCfg ξ (⟦ m ⟧ₘ k) := renameA.right m k
+theorem renameAval {ξ v} : ⟦ renameVal ξ v ⟧ᵥ = ANF.renameVal ξ ⟦ v ⟧ᵥ := renameA.left v
+theorem renameAcom {ξ m k} : (⟦ renameCom ξ m ⟧ₘ ANF.renameK ξ k) = ANF.renameCfg ξ (⟦ m ⟧ₘ k) := renameA.right m k
 
 /-* Substitution commutes with translation *-/
 
-theorem substAupCfg {σ m} : ANF.substCfg (⟦ ⇑ σ ⟧ₛ) m = ANF.substCfg (⇑ (⟦ σ ⟧ₛ)) m := by
+theorem substAupCfg {σ m} : ANF.substCfg ⟦ ⇑ σ ⟧ₛ m = ANF.substCfg (⇑ ⟦ σ ⟧ₛ) m := by
   apply ANF.substCfgExt; intro n; cases n <;> simp [renameAval]
 
-theorem substAupK {σ k} : ANF.substK (⟦ ⇑ σ ⟧ₛ) k = ANF.substK (⇑ (⟦ σ ⟧ₛ)) k := by
+theorem substAupK {σ k} : ANF.substK ⟦ ⇑ σ ⟧ₛ k = ANF.substK (⇑ ⟦ σ ⟧ₛ) k := by
   apply ANF.substKExt; intro n; cases n <;> simp [renameAval]
 
 theorem substA {σ} :
-  (∀ v, (⟦ substVal σ v ⟧ᵥ) = ANF.substVal (⟦ σ ⟧ₛ) (⟦ v ⟧ᵥ)) ∧
-  (∀ m k, (⟦ substCom σ m ⟧ₘ (ANF.substK (⟦ σ ⟧ₛ) k)) = ANF.substCfg (⟦ σ ⟧ₛ) (⟦ m ⟧ₘ k)) := by
+  (∀ v, ⟦ substVal σ v ⟧ᵥ = ANF.substVal ⟦ σ ⟧ₛ ⟦ v ⟧ᵥ) ∧
+  (∀ m k, (⟦ substCom σ m ⟧ₘ ANF.substK ⟦ σ ⟧ₛ k) = ANF.substCfg ⟦ σ ⟧ₛ (⟦ m ⟧ₘ k)) := by
   refine ⟨λ v ↦ ?val, λ m k ↦ ?com⟩
   mutual_induction v, m generalizing σ
   case var | unit => rfl
@@ -563,13 +623,31 @@ theorem substA {σ} :
   case letin ihn ihm =>
     simp [-lift, -up, -ANF.up, ← ihn, ← substAupCfg, ← ihm, ANF.substKLiftSucc, substAupK]
   case case ihv ihm₁ ihm₂ =>
-    have eσ {σ} : (.var 0 +: ANF.renameVal succ ∘ σ) = (⇑ σ) := rfl
+    have eσ {σ} : (.var 0 +: ANF.renameVal succ ∘ σ) = ⇑ σ := rfl
     simp [-lift, -up, -ANF.up, ihv, ANF.substKLiftSucc, ← substAupCfg, ← substAupK, ihm₁, ihm₂]
   case prod ihm₁ ihm₂ => simp [← ihm₁, ← ihm₂, ANF.substPlug]
   case fst ih | snd ih => simp [← ih]
 
-theorem substAval {σ v} : (⟦ substVal σ v ⟧ᵥ) = ANF.substVal (⟦ σ ⟧ₛ) (⟦ v ⟧ᵥ) := substA.left v
-theorem substAcom {σ m k} : (⟦ substCom σ m ⟧ₘ (ANF.substK (⟦ σ ⟧ₛ) k)) = ANF.substCfg (⟦ σ ⟧ₛ) (⟦ m ⟧ₘ k) := substA.right m k
+theorem substAval {σ v} : ⟦ substVal σ v ⟧ᵥ = ANF.substVal ⟦ σ ⟧ₛ ⟦ v ⟧ᵥ := substA.left v
+theorem substAcom {σ m k} : (⟦ substCom σ m ⟧ₘ ANF.substK ⟦ σ ⟧ₛ k) = ANF.substCfg ⟦ σ ⟧ₛ (⟦ m ⟧ₘ k) := substA.right m k
+
+theorem substAcomOne {m : Com} {v : Val} {k} : ANF.substCfg (⟦ v ⟧ᵥ +: .var) (⟦ m ⟧ₘ ANF.renameK succ k) = (⟦ m⦃v⦄ ⟧ₘ k) := by
+  calc ANF.substCfg (⟦ v ⟧ᵥ +: .var) (⟦ m ⟧ₘ ANF.renameK succ k)
+    _ = ANF.substCfg (⟦ v +: .var ⟧ₛ) (⟦ m ⟧ₘ ANF.renameK succ k)  := by rw [ANF.substCfgExt (λ n ↦ ?_)]; cases n <;> simp
+    _ = ⟦ m⦃v⦄ ⟧ₘ (ANF.substK ⟦ v +: .var ⟧ₛ (ANF.renameK succ k)) := Eq.symm substAcom
+    _ = ⟦ m⦃v⦄ ⟧ₘ (ANF.substK (⟦ v +: .var ⟧ₛ ∘ succ) k)           := by rw [ANF.substRenameK]
+    _ = ⟦ m⦃v⦄ ⟧ₘ (ANF.substK .var k)                              := by rw [ANF.substKExt (λ n ↦ ?_)]; cases n <;> simp
+    _ = ⟦ m⦃v⦄ ⟧ₘ k                                                := by rw [ANF.substKId]
+
+/-* Continuation composition commutes with translation *-/
+
+theorem compA {m k₁ k₂} : ANF.compKCfg k₁ (⟦ m ⟧ₘ k₂) = ⟦ m ⟧ₘ ANF.compKK k₁ k₂ := by
+  mutual_induction m generalizing k₁ k₂
+  case force | lam | ret => exact ANF.compPlug
+  case app ih | fst ih | snd ih => simp [ih]
+  case letin ihn ihm => simp [ihn, ihm, ANF.renameCompKK]
+  case case ihm₁ ihm₂ => simp [ihm₁, ihm₂, ANF.renameCompKK]
+  case prod ihm₁ ihm₂ => simp [ihm₁, ihm₂, ANF.compPlug]
 
 /-* CK machine semantics of ANF *-/
 
@@ -621,19 +699,19 @@ end ANF
 @[simp]
 def SK : S → ANF.K
   | [] => .nil
-  | .app v :: k => .app (⟦ v ⟧ᵥ) (SK k)
-  | .letin m :: k => .letin (⟦ m ⟧ₘ (ANF.renameK succ (SK k)))
+  | .app v :: k => .app ⟦ v ⟧ᵥ (SK k)
+  | .letin m :: k => .letin (⟦ m ⟧ₘ ANF.renameK succ (SK k))
   | .fst :: k => .fst (SK k)
   | .snd :: k => .snd (SK k)
 
 @[simp]
 def SSₐ : S → ANF.Sₐ
   | [] => []
-  | .app v :: k => .app (⟦ v ⟧ᵥ) :: SSₐ k
-  | .letin m :: k => .letin (⟦ m ⟧ₘ) :: SSₐ k
+  | .app v :: k => .app ⟦ v ⟧ᵥ :: SSₐ k
+  | .letin m :: k => .letin ⟦ m ⟧ₘ :: SSₐ k
   | .fst :: k => .fst :: SSₐ k
   | .snd :: k => .snd :: SSₐ k
-notation:40 "⟦" k:41 "⟧ₛₛ" => SSₐ k
+notation:1023 "⟦" k:41 "⟧ₛₛ" => SSₐ k
 
 theorem renameSK {k} (ξ : Nat → Nat) : SK (renameS ξ k) = ANF.renameK ξ (SK k) := by
   induction k
@@ -641,7 +719,7 @@ theorem renameSK {k} (ξ : Nat → Nat) : SK (renameS ξ k) = ANF.renameK ξ (SK
   case cons f _ ih =>
     cases f <;> simp [-lift, ih, renameAval, ← renameAcom, ← ANF.renameKLiftSucc]
 
-theorem renameSSₐ {k} (ξ : Nat → Nat) : (⟦ renameS ξ k ⟧ₛₛ) = ANF.renameKₐ ξ (⟦ k ⟧ₛₛ) := by
+theorem renameSSₐ {k} (ξ : Nat → Nat) : ⟦ renameS ξ k ⟧ₛₛ = ANF.renameKₐ ξ ⟦ k ⟧ₛₛ := by
   induction k
   case nil => simp
   case cons f _ ih =>
@@ -666,15 +744,15 @@ theorem CKeqv₁ {m₁ m₂ f} {k : S} (r : ⟨m₁, f :: k⟩ ⤳ ⟨m₂, k⟩
   all_goals try cases loopK₂ e
   all_goals injection e with ef ek; subst ef; clear ek
   case β m v =>
-    calc ⟨.com (.lam (⟦ m ⟧ₘ .nil)), .app (⟦ v ⟧ᵥ) :: (⟦ k ⟧ₛₛ)⟩
-      _ ⤳ ⟨ANF.substCfg ((⟦ v ⟧ᵥ) +: .var) (⟦ m ⟧ₘ .nil), ⟦ k ⟧ₛₛ⟩ := .β
-      _ = ⟨ANF.substCfg (⟦ v +: .var ⟧ₛ) (⟦ m ⟧ₘ .nil), ⟦ k ⟧ₛₛ⟩   := by rw [ANF.substCfgExt (λ n ↦ ?_)]; cases n <;> rfl
-      _ = ⟨⟦ m⦃v⦄ ⟧ₘ .nil, ⟦ k ⟧ₛₛ⟩                                := by rw [← substAcom]; rfl
+    calc ⟨.com (.lam ⟦ m ⟧ₘ), .app ⟦ v ⟧ᵥ :: ⟦ k ⟧ₛₛ⟩
+      _ ⤳ ⟨ANF.substCfg (⟦ v ⟧ᵥ +: .var) ⟦ m ⟧ₘ, ⟦ k ⟧ₛₛ⟩ := .β
+      _ = ⟨ANF.substCfg ⟦ v +: .var ⟧ₛ ⟦ m ⟧ₘ, ⟦ k ⟧ₛₛ⟩    := by rw [ANF.substCfgExt (λ n ↦ ?_)]; cases n <;> rfl
+      _ = ⟨⟦ m⦃v⦄ ⟧ₘ, ⟦ k ⟧ₛₛ⟩                             := by rw [← substAcom]; rfl
   case ζ v m =>
-    calc ⟨.com (.ret (⟦ v ⟧ᵥ)), .letin (⟦ m ⟧ₘ) :: (⟦ k ⟧ₛₛ)⟩
-      _ ⤳ ⟨ANF.substCfg ((⟦ v ⟧ᵥ) +: .var) (⟦ m ⟧ₘ), ⟦ k ⟧ₛₛ⟩ := .ζ
-      _ = ⟨ANF.substCfg (⟦ v +: .var ⟧ₛ) (⟦ m ⟧ₘ), ⟦ k ⟧ₛₛ⟩   := by rw [ANF.substCfgExt (λ n ↦ ?_)]; cases n <;> rfl
-      _ = ⟨⟦ m⦃v⦄ ⟧ₘ .nil, ⟦ k ⟧ₛₛ⟩                           := by rw [← substAcom]; rfl
+    calc ⟨.com (.ret ⟦ v ⟧ᵥ), .letin ⟦ m ⟧ₘ :: ⟦ k ⟧ₛₛ⟩
+      _ ⤳ ⟨ANF.substCfg (⟦ v ⟧ᵥ +: .var) ⟦ m ⟧ₘ, ⟦ k ⟧ₛₛ⟩ := .ζ
+      _ = ⟨ANF.substCfg ⟦ v +: .var ⟧ₛ ⟦ m ⟧ₘ, ⟦ k ⟧ₛₛ⟩    := by rw [ANF.substCfgExt (λ n ↦ ?_)]; cases n <;> rfl
+      _ = ⟨⟦ m⦃v⦄ ⟧ₘ .nil, ⟦ k ⟧ₛₛ⟩                        := by rw [← substAcom]; rfl
   case π1 | π2 => constructor
 
 theorem CKeqv₂ {m₁ m₂} {k : S} (r : ⟨m₁, k⟩ ⤳ ⟨m₂, k⟩) : ⟨⟦ m₁ ⟧ₘ, ⟦ k ⟧ₛₛ⟩ ⤳ ⟨⟦ m₂ ⟧ₘ, ⟦ k ⟧ₛₛ⟩ := by
@@ -685,15 +763,15 @@ theorem CKeqv₂ {m₁ m₂} {k : S} (r : ⟨m₁, k⟩ ⤳ ⟨m₂, k⟩) : ⟨
   all_goals try cases loopK₁ (Eq.symm ek)
   case π => constructor
   case ιl v m₁ m₂ =>
-    calc ⟨.case (.inl (⟦ v ⟧ᵥ)) (⟦ m₁ ⟧ₘ .nil) (⟦ m₂ ⟧ₘ .nil), ⟦ k ⟧ₛₛ⟩
-      _ ⤳ ⟨ANF.substCfg ((⟦ v ⟧ᵥ) +: .var) (⟦ m₁ ⟧ₘ .nil), ⟦ k ⟧ₛₛ⟩ := .ιl
-      _ = ⟨ANF.substCfg (⟦ v +: .var ⟧ₛ) (⟦ m₁ ⟧ₘ .nil), ⟦ k ⟧ₛₛ⟩   := by rw [ANF.substCfgExt (λ n ↦ ?_)]; cases n <;> rfl
-      _ = ⟨⟦ m₁⦃v⦄ ⟧ₘ .nil, ⟦ k ⟧ₛₛ⟩                                := by rw [← substAcom]; rfl
+    calc ⟨.case (.inl ⟦ v ⟧ᵥ) ⟦ m₁ ⟧ₘ ⟦ m₂ ⟧ₘ, ⟦ k ⟧ₛₛ⟩
+      _ ⤳ ⟨ANF.substCfg (⟦ v ⟧ᵥ +: .var) ⟦ m₁ ⟧ₘ, ⟦ k ⟧ₛₛ⟩ := .ιl
+      _ = ⟨ANF.substCfg ⟦ v +: .var ⟧ₛ ⟦ m₁ ⟧ₘ, ⟦ k ⟧ₛₛ⟩    := by rw [ANF.substCfgExt (λ n ↦ ?_)]; cases n <;> rfl
+      _ = ⟨⟦ m₁⦃v⦄ ⟧ₘ, ⟦ k ⟧ₛₛ⟩                             := by rw [← substAcom]; rfl
   case ιr v m₁ m₂ =>
-    calc ⟨.case (.inr (⟦ v ⟧ᵥ)) (⟦ m₁ ⟧ₘ .nil) (⟦ m₂ ⟧ₘ .nil), ⟦ k ⟧ₛₛ⟩
-      _ ⤳ ⟨ANF.substCfg ((⟦ v ⟧ᵥ) +: .var) (⟦ m₂ ⟧ₘ .nil), ⟦ k ⟧ₛₛ⟩ := .ιr
-      _ = ⟨ANF.substCfg (⟦ v +: .var ⟧ₛ) (⟦ m₂ ⟧ₘ .nil), ⟦ k ⟧ₛₛ⟩   := by rw [ANF.substCfgExt (λ n ↦ ?_)]; cases n <;> rfl
-      _ = ⟨⟦ m₂⦃v⦄ ⟧ₘ .nil, ⟦ k ⟧ₛₛ⟩                                := by rw [← substAcom]; rfl
+    calc ⟨.case (.inr ⟦ v ⟧ᵥ) ⟦ m₁ ⟧ₘ ⟦ m₂ ⟧ₘ, ⟦ k ⟧ₛₛ⟩
+      _ ⤳ ⟨ANF.substCfg (⟦ v ⟧ᵥ +: .var) ⟦ m₂ ⟧ₘ, ⟦ k ⟧ₛₛ⟩ := .ιr
+      _ = ⟨ANF.substCfg ⟦ v +: .var ⟧ₛ ⟦ m₂ ⟧ₘ, ⟦ k ⟧ₛₛ⟩    := by rw [ANF.substCfgExt (λ n ↦ ?_)]; cases n <;> rfl
+      _ = ⟨⟦ m₂⦃v⦄ ⟧ₘ, ⟦ k ⟧ₛₛ⟩                             := by rw [← substAcom]; rfl
 
 theorem CKeqv₃ {m₁ m₂ f} {k : S} (r : ⟨m₁, k⟩ ⤳ ⟨m₂, f :: k⟩) : (⟦ m₁ ⟧ₘ SK k) = (⟦ m₂ ⟧ₘ SK (f :: k)) := by
   generalize e : f :: k = k' at r
@@ -702,46 +780,281 @@ theorem CKeqv₃ {m₁ m₂ f} {k : S} (r : ⟨m₁, k⟩ ⤳ ⟨m₂, f :: k⟩
   all_goals try cases loopK₂ e
   all_goals rfl
 
-/-* Composing continuations *-/
+/-* Equational theory of ANF *-/
 
-/-
+namespace ANF
+section
+set_option hygiene false
+local infix:40 "≡ᵥ" => EqVal
+local infix:40 "≡ₙ" => EqCom
+local infix:40 "≡ₘ" => EqCfg
+mutual
+inductive EqVal : Val → Val → Prop
+  | var {x} : .var x ≡ᵥ .var x
+  | unit : .unit ≡ᵥ .unit
+  | inl {v w} : v ≡ᵥ w → .inl v ≡ᵥ .inl w
+  | inr {v w} : v ≡ᵥ w → .inr v ≡ᵥ .inr w
+  | thunk {m n} : m ≡ₘ n → .thunk m ≡ᵥ .thunk n
+  | sym {v w} : w ≡ᵥ v → v ≡ᵥ w
+  | trans {u v w} : u ≡ᵥ v → v ≡ᵥ w → u ≡ᵥ w
+
+inductive EqCom : Com → Com → Prop
+  | force {v w} : v ≡ᵥ w → .force v ≡ₙ .force w
+  | lam {m n} : m ≡ₘ n → .lam m ≡ₙ .lam n
+  | app {m n v w} : m ≡ₙ n → v ≡ᵥ w → .app m v ≡ₙ .app n w
+  | ret {v w} : v ≡ᵥ w → .ret v ≡ₙ .ret w
+  | prod {m₁ m₂ n₁ n₂} : m₁ ≡ₘ n₁ → m₂ ≡ₘ n₂ → .prod m₁ m₂ ≡ₙ .prod n₁ n₂
+  | fst {m n} : m ≡ₙ n → .fst m ≡ₙ .fst n
+  | snd {m n} : m ≡ₙ n → .snd m ≡ₙ .snd n
+  | sym {m n} : n ≡ₙ m → m ≡ₙ n
+  | trans {m n p} : m ≡ₙ n → n ≡ₙ p → m ≡ₙ p
+
+inductive EqCfg : Cfg → Cfg → Prop
+  | com {m n} : m ≡ₙ n → .com m ≡ₘ .com n
+  | letin {m₁ m₂ n₁ n₂} : m₁ ≡ₙ n₁ → m₂ ≡ₘ n₂ → .letin m₁ m₂ ≡ₘ .letin n₁ n₂
+  | case {v w m₁ n₁ m₂ n₂} : v ≡ᵥ w → m₁ ≡ₘ n₁ → m₂ ≡ₘ n₂ → .case v m₁ m₂ ≡ₘ .case w n₁ n₂
+  | β {m v} : .com (.app (.lam m) v) ≡ₘ substCfg (v +: .var) m
+  | π {m} : .com (.force (.thunk m)) ≡ₘ m
+  | π1 {m₁ m₂} : .com (.fst (.prod m₁ m₂)) ≡ₘ m₁
+  | π2 {m₁ m₂} : .com (.snd (.prod m₁ m₂)) ≡ₘ m₂
+  | ζ {m v} : .letin (.ret v) m ≡ₘ substCfg (v +: .var) m
+  | ιl {v m₁ m₂} : .case (.inl v) m₁ m₂ ≡ₘ substCfg (v +: .var) m₁
+  | ιr {v m₁ m₂} : .case (.inr v) m₁ m₂ ≡ₘ substCfg (v +: .var) m₂
+  | sym {m n} : n ≡ₘ m → m ≡ₘ n
+  | trans {m n p} : m ≡ₘ n → n ≡ₘ p → m ≡ₘ p
+end
+end
+infix:40 "≡ᵥ" => EqVal
+infix:40 "≡ₙ" => EqCom
+infix:40 "≡ₘ" => EqCfg
+
+theorem reflValCom :
+  (∀ {v : Val}, v ≡ᵥ v) ∧
+  (∀ {n : Com}, n ≡ₙ n) ∧
+  (∀ {m : Cfg}, m ≡ₘ m) := by
+  refine ⟨λ {v} ↦ ?val, λ {n} ↦ ?com, λ {m} ↦ ?cfg⟩
+  mutual_induction v, n, m
+  all_goals constructor <;> assumption
+
+@[refl] theorem EqVal.refl : ∀ {v : Val}, v ≡ᵥ v := reflValCom.left
+@[refl] theorem EqCom.refl : ∀ {n : Com}, n ≡ₙ n := reflValCom.right.left
+@[refl] theorem EqCfg.refl : ∀ {m : Cfg}, m ≡ₘ m := reflValCom.right.right
+
+instance : Trans EqVal EqVal EqVal where
+  trans := .trans
+
+instance : Trans EqCom EqCom EqCom where
+  trans := .trans
+
+instance : Trans EqCfg EqCfg EqCfg where
+  trans := .trans
+
+theorem EqCom.plug {n₁ n₂ k} (e : n₁ ≡ₙ n₂) : (k [ n₁ ]) ≡ₘ (k [ n₂ ]) := by
+  induction k generalizing n₁ n₂
+  case' app ih | fst ih | snd ih => apply ih
+  all_goals constructor; assumption; try rfl
+
+theorem EqCom.compK {n m k} (e : .com n ≡ₘ m) : (k [ n ]) ≡ₘ compKCfg k m := by
+  mutual_induction m generalizing n k
+  case com => apply EqCom.plug; sorry
+  case letin => simp; sorry
+  case case ihm₁ ihm₂ => simp; sorry
+
+end ANF
+
+theorem waaaahEq :
+  (∀ {v w : Val}, v ≡ w → ⟦ v ⟧ᵥ ≡ᵥ ⟦ w ⟧ᵥ) ∧
+  (∀ {k} {m n : Com}, m ≡ n → (⟦ m ⟧ₘ k) ≡ₘ (⟦ n ⟧ₘ k)) := by
+  refine ⟨λ ev ↦ ?eqval, λ em ↦ ?eqcom⟩
+  mutual_induction ev, em
+  case var | unit | inl ih | inr ih | thunk ih =>
+    constructor; try simp [ih]
+  case force | lam | ret | prod =>
+    apply ANF.EqCom.plug; constructor <;> apply_assumption
+  case case ihv ihm₁ ihm₂ _ => constructor <;> apply_assumption
+  case app ihm ihv _ | letin ihn ihm _ => simp; sorry -- equality of continuations
+  case fst ih _ | snd ih _ => exact ih
+  case eqval.sym e => exact .sym e
+  case eqval.trans e₁ e₂ => exact .trans e₁ e₂
+  case eqcom.sym e _ => exact .sym e
+  case eqcom.trans e₁ e₂ _ => exact .trans e₁ e₂
+  case β k =>
+    have eknil (k : ANF.K) : k = ANF.compKK k .nil := by rfl
+    rw [eknil k, ← compA, ← compA]; simp
+    apply ANF.EqCom.compK
+    rw [← substAcomOne]; simp
+    constructor
+  case ζ k => rw [← substAcomOne]; constructor
+  case π k | π1 k | π2 k =>
+    have eknil (k : ANF.K) : k = ANF.compKK k .nil := by rfl
+    simp; rw [eknil k, ← compA]
+    apply ANF.EqCom.compK
+    constructor
+  case ιl v m₁ m₂ k => rw [← substAcomOne]; exact .ιl
+  case ιr v m₁ m₂ k => rw [← substAcomOne]; exact .ιr
+
+/-* Big step semantics of ANF *-/
+
+namespace ANF
+
+section
+set_option hygiene false
+local infix:40 "⇓" => StepCom
+local infix:40 "⇓" => StepCfg
+mutual
+inductive StepCom : Com → Com → Prop where
+  | lam {m : Cfg} : .lam m ⇓ .lam m
+  | ret {v : Val} : .ret v ⇓ .ret v
+  | prod {m₁ m₂ : Cfg} : .prod m₁ m₂ ⇓ .prod m₁ m₂
+  | π {m : Cfg} {t} :
+    m ⇓ t →
+    ---------------------
+    .force (.thunk m) ⇓ t
+  | β {n t : Com} {m v} :
+    n ⇓ .lam m →
+    substCfg (v +: .var) m ⇓ t →
+    -----------------------------
+    .app n v ⇓ t
+  | π1 {n t : Com} {m₁ m₂} :
+    n ⇓ .prod m₁ m₂ →
+    m₁ ⇓ t →
+    -----------
+    .fst n ⇓ t
+  | π2 {n t : Com} {m₁ m₂} :
+    n ⇓ .prod m₁ m₂ →
+    m₂ ⇓ t →
+    -----------
+    .snd n ⇓ t
+
+inductive StepCfg : Cfg → Com → Prop where
+  | com {n t : Com} : n ⇓ t → .com n ⇓ t
+  | ζ {n t : Com} {v m} :
+    n ⇓ .ret v →
+    substCfg (v +: .var) m ⇓ t →
+    -----------------------------
+    .letin n m ⇓ t
+  | ιl {v m₁ m₂ t}:
+    substCfg (v +: .var) m₁ ⇓ t →
+    -----------------------------
+    .case (.inl v) m₁ m₂ ⇓ t
+  | ιr {v m₁ m₂ t}:
+    substCfg (v +: .var) m₂ ⇓ t →
+    -----------------------------
+    .case (.inr v) m₁ m₂ ⇓ t
+end
+end
+infix:40 "⇓" => StepCom
+infix:40 "⇓" => StepCfg
+
 @[simp]
-def compKCfg (k : ANF.K) : ANF.Cfg → ANF.Cfg
-  | .com n => ANF.plug n k
-  | .letin n m => .letin n (compKCfg (ANF.renameK succ k) m)
-  | .case v m₁ m₂ => .case v (compKCfg (ANF.renameK succ k) m₁) (compKCfg (ANF.renameK succ k) m₂)
+def isTerminal : Com → Prop
+  | .lam _ | .ret _ | .prod _ _ => True
+  | _ => False
+
+theorem stepTerminal {t} :
+  (∀ {n : Com}, n ⇓ t → isTerminal t) ∧
+  (∀ {m : Cfg}, m ⇓ t → isTerminal t) := by
+  refine ⟨λ {n} r ↦ ?com, λ {m} r ↦ ?cfg⟩
+  mutual_induction r, r
+  case lam | ret | prod => constructor
+  all_goals assumption
+
+theorem StepCfg.compK {m : Cfg} {n t : Com} {k} (h : ∀ t, m ⇓ t → n ⇓ t) (b : compKCfg k m ⇓ t) : (k [ n ]) ⇓ t := by
+  mutual_induction n generalizing m t
+  case app => sorry
+  all_goals sorry
+end ANF
+
+theorem waaahBig {m₁ m₂ : Com} {k₁ k₂ t} (r : ⟨m₁, k₁⟩ ⤳ ⟨m₂, k₂⟩) (b : (⟦ m₂ ⟧ₘ SK k₂) ⇓ t) : (⟦ m₁ ⟧ₘ SK k₁) ⇓ t := by
+  generalize e₁ : (m₁, k₁) = ck₁ at r
+  generalize e₂ : (m₂, k₂) = ck₂ at r
+  induction r
+  all_goals injection e₁ with em ek; subst em ek
+  all_goals injection e₂ with em ek; subst em ek
+  case β => simp; sorry
+  all_goals sorry
+
+/-* Failed proofs *-/
 
 @[simp]
-def compKK (k : ANF.K) : ANF.K → ANF.K
-  | .nil => k
-  | .app v k' => .app v (compKK k k')
-  | .letin m => .letin (compKCfg (ANF.renameK succ k) m)
-  | .fst k' => .fst (compKK k k')
-  | .snd k' => .snd (compKK k k')
+def SₐK : ANF.Sₐ → ANF.K
+  | [] => .nil
+  | .app v :: k => .app v (SₐK k)
+  | .letin m :: k => .letin (ANF.compKCfg (SₐK k) m)
+  | .fst :: k => .fst (SₐK k)
+  | .snd :: k => .snd (SₐK k)
 
-theorem renameCompKCfg {ξ m k} : ANF.renameCfg ξ (compKCfg k m) = compKCfg (ANF.renameK ξ k) (ANF.renameCfg ξ m) := by
-  mutual_induction m generalizing ξ k
-  case com => simp [ANF.renamePlug]
-  case letin ih => simp [ih, ANF.renameKLiftSucc]
-  case case ihm₁ ihm₂ => simp [ihm₁, ihm₂, ANF.renameKLiftSucc]
+theorem CKeqv' {m₁ m₂} {k₁ : S} (r : ⟨m₁, k₁⟩ ⤳⋆ ⟨m₂, []⟩) : ∃ m k, ⟨m, k⟩ ⤳⋆ ⟨⟦ m₂ ⟧ₘ, []⟩ ∧ (⟦ m₁ ⟧ₘ SK k₁) = (ANF.compKCfg (SₐK k) m) := by
+  generalize e₁ : (m₁, k₁) = ck₁ at r
+  generalize e₂ : (m₂, []) = ck₂ at r
+  induction r generalizing m₁ m₂ k₁
+  case refl =>
+    subst e₁; injection e₂ with em ek; subst em ek
+    exists ⟦ m₂ ⟧ₘ, []; simp [ANF.compKCfgNil]; rfl
+  case trans ck _ r _ ih =>
+    subst e₁ e₂
+    let ⟨m', k', r', e⟩ := ih rfl rfl
+    cases r
+    case β m v k r =>
+      simp at *
+      exists .com (.lam ⟦ m ⟧ₘ), .app ⟦ v ⟧ᵥ :: ⟦ k ⟧ₛₛ
+      constructor
+      apply RTC.trans' ?_ r'
+      all_goals sorry
+    all_goals sorry
 
-theorem renameCompKK {ξ k₁ k₂} : ANF.renameK ξ (compKK k₁ k₂) = compKK (ANF.renameK ξ k₁) (ANF.renameK ξ k₂) := by
-  induction k₂
-  case nil => simp
-  case app ih | fst ih | snd ih => simp [ih]
-  case letin => simp [ANF.renameKLiftSucc, renameCompKCfg]
+theorem appendNil {α} {xs : List α} : xs = xs ++ [] := by
+  induction xs <;> simp
 
-theorem compPlug {n k₁ k₂} : compKCfg k₁ (k₂ [ n ]) = ((compKK k₁ k₂) [ n ]) := by
-  induction k₂ generalizing n <;> apply_assumption
+theorem CKeqv'' {m₁ m₂ : Com} {k₁ k₂} (r : ⟨m₁, k₁⟩ ⤳ ⟨m₂, k₂⟩) :
+  ∃ k₁₁ k₁₂ k₂₁ k₂₂,
+    ⟨⟦ m₁ ⟧ₘ SK k₁₁, k₁₂⟩ ⤳⋆ ⟨⟦ m₂ ⟧ₘ SK k₂₁, k₂₂⟩ ∧
+    ⟦ k₁ ⟧ₛₛ = ⟦ k₁₁ ⟧ₛₛ ++ k₁₂ ∧
+    ⟦ k₂ ⟧ₛₛ = ⟦ k₂₁ ⟧ₛₛ ++ k₂₂ := by
+  generalize e₁ : (m₁, k₁) = ck₁ at r
+  generalize e₂ : (m₂, k₂) = ck₂ at r
+  induction r
+  all_goals injection e₁ with em ek; subst em ek
+  all_goals injection e₂ with em ek; subst em ek
+  case β m v =>
+    exact ⟨.nil, ⟦ .app v :: k₂ ⟧ₛₛ, .nil, _, .once (CKeqv₁ .β), rfl, rfl⟩
+  case app v =>
+    refine ⟨_, .nil, .app v :: k₁ , .nil, by rw [CKeqv₃ .app], appendNil, appendNil⟩
+  all_goals sorry
 
-theorem compA {m k₁ k₂} : compKCfg k₁ (⟦ m ⟧ₘ k₂) = (⟦ m ⟧ₘ (compKK k₁ k₂)) := by
-  mutual_induction m generalizing k₁ k₂
-  case force | lam | ret => exact compPlug
-  case app ih | fst ih | snd ih => simp [ih]
-  case letin ihn ihm => simp [ihn, ihm, renameCompKK]
-  case case ihm₁ ihm₂ => simp [ihm₁, ihm₂, renameCompKK]
-  case prod ihm₁ ihm₂ => simp [ihm₁, ihm₂, compPlug]
--/
+theorem CKeqv''' {m₁ m₂ : Com} {k₁ k₂} (r : ⟨m₁, k₁⟩ ⤳⋆ ⟨m₂, k₂⟩) :
+  ∃ k₁₁ k₁₂ k₂₁ k₂₂,
+    ⟨⟦ m₁ ⟧ₘ SK k₁₁, k₁₂⟩ ⤳⋆ ⟨⟦ m₂ ⟧ₘ SK k₂₁, k₂₂⟩ ∧
+    ⟦ k₁ ⟧ₛₛ = ⟦ k₁₁ ⟧ₛₛ ++ k₁₂ ∧
+    ⟦ k₂ ⟧ₛₛ = ⟦ k₂₁ ⟧ₛₛ ++ k₂₂ := by
+  generalize e₁ : (m₁, k₁) = ck₁ at r
+  generalize e₂ : (m₂, k₂) = ck₂ at r
+  induction r generalizing m₁ k₁
+  case refl =>
+    subst e₁; injection e₂ with em ek; subst em ek
+    exists k₂, .nil, k₂, .nil
+    rw [← appendNil]; simp; rfl
+  case trans ck _ r _ ih =>
+    subst e₁ e₂
+    match ck with
+    | .mk m₂ k₂ =>
+    match ih rfl rfl with
+    | ⟨_, _, _, _, r₂, e₁, e₂⟩ =>
+    refine ⟨?_, ?_, _, _, RTC.trans' ?_ r₂, ?_, e₂⟩
+    all_goals sorry
+
+theorem CKeqv'''' {m₁ m₂} {k : S} (r : ⟨m₁, k⟩ ⤳⋆ ⟨m₂, []⟩) :
+  ∃ k₁ k₂, ⟨⟦ m₁ ⟧ₘ SK k₁, k₂⟩ ⤳⋆ ⟨⟦ m₂ ⟧ₘ, []⟩ ∧ (⟦ k ⟧ₛₛ) = (⟦ k₁ ⟧ₛₛ) ++ k₂ := by
+  generalize e₁ : (m₁, k) = ck₁ at r
+  generalize e₂ : (m₂, []) = ck₂ at r
+  induction r generalizing m₁ k
+  case refl =>
+    subst e₁; injection e₂ with em ek; subst em ek
+    exists .nil, []
+  case trans ck₁ _ r _ ih =>
+    subst e₁ e₂
+    match ck₁ with
+    | .mk m₂ k₂ => sorry
 
 /-
 @[simp]
